\documentclass{article}
\usepackage{amsmath}
\usepackage[margin=2cm]{geometry}

\begin{document}

\begin{align}
A(D) &= \frac{\Delta H_{\rm v} \rho_{\rm w}}{4 k_{\rm a}'(D) T_{\infty}} \\
B(D) &= \frac{4 D_{\rm v}'(D) M_{\rm w} P^{\rm 0}(T_{\infty})}{\rho_w R T_{\infty}} \\
C &= \frac{\Delta H_{\rm v} M_{\rm w}}{R T_{\infty}} \\
E(D) &= \frac{4 M_{\rm w}\sigma_{\rm w}}{R T_{\infty} \rho_{\rm w} D} \\
\delta &= A D \frac{d D}{dt} \\
k_{\rm a}'(D) &= \frac{k_{\rm a}}{1 + \frac{2 k_{\rm a}}{\alpha D \rho_{\rm air} c_{\rm p,w}} \sqrt{\frac{2 \pi M_{\rm air}}{R T}}} \\
D_{\rm v}'(D) &= \frac{D_{\rm v}}{1 + \frac{2 D_{\rm v}}{\alpha D} \sqrt{\frac{2 \pi M_{\rm w}}{R T}}} \\
a_{\rm w}(D) &= \frac{\frac{\pi}{6}(D)^{3}-V_{\rm s}}{\frac{\pi}{6}(D)^{3}+(\kappa-1)V_{\rm s}}
\end{align}

\begin{equation}
  f(\delta, D) = \frac{\delta}{A(D)}
  - B(D) \Bigg(S-\left(\frac{\delta}{1+\delta}\right)
  a_{\rm w}(D)
  \exp{\left(C \frac{\delta}{1+\delta} + E(D) \frac{1}{1+\delta}\right)} \Bigg)
\end{equation}

\begin{align}
  0 &= f(\delta^*(D), D) \\
  0 &= \frac{d}{d D} f(\delta^*(D), D) \\
  &= \frac{\partial f}{\partial \delta}(\delta^*(D), D)
  \frac{\partial \delta^*}{\partial D}(D)
  + \frac{\partial f}{\partial D}(\delta^*(D), D) \\
  \frac{\partial \delta^*}{\partial D}(D)
  &= - \frac{\frac{\partial f}{\partial D}(\delta^*(D), D)}{\frac{\partial f}{\partial \delta}(\delta^*(D), D)}
\end{align}

\end{document}
